theories/AutoSubst/Ast.v
@@ -21,6 +21,7 @@ Inductive term : Type :=
   | tTrue : term
   | tFalse : term
   | tBoolElim : term -> term -> term -> term -> term
+  | tAlpha : term -> term
   | tEmpty : term
   | tEmptyElim : term -> term -> term
   | tSig : term -> term -> term
@@ -115,6 +116,12 @@ exact (eq_trans
                (ap (fun x => tBoolElim t0 x s2 s3) H1))
             (ap (fun x => tBoolElim t0 t1 x s3) H2))
          (ap (fun x => tBoolElim t0 t1 t2 x) H3)).
+Qed.
+
+Lemma congr_tAlpha {s0 : term} {t0 : term} (H0 : s0 = t0) :
+  tAlpha s0 = tAlpha t0.
+Proof.
+exact (eq_trans eq_refl (ap (fun x => tAlpha x) H0)).
 Qed.
 
 Lemma congr_tEmpty : tEmpty = tEmpty.
@@ -221,6 +228,7 @@ Fixpoint ren_term (xi_term : nat -> nat) (s : term) {struct s} : term :=
   | tBoolElim s0 s1 s2 s3 =>
       tBoolElim (ren_term (upRen_term_term xi_term) s0) (ren_term xi_term s1)
         (ren_term xi_term s2) (ren_term xi_term s3)
+  | tAlpha s0 => tAlpha (ren_term xi_term s0)
   | tEmpty => tEmpty
   | tEmptyElim s0 s1 =>
       tEmptyElim (ren_term (upRen_term_term xi_term) s0)
@@ -272,6 +280,7 @@ term :=
       tBoolElim (subst_term (up_term_term sigma_term) s0)
         (subst_term sigma_term s1) (subst_term sigma_term s2)
         (subst_term sigma_term s3)
+  | tAlpha s0 => tAlpha (subst_term sigma_term s0)
   | tEmpty => tEmpty
   | tEmptyElim s0 s1 =>
       tEmptyElim (subst_term (up_term_term sigma_term) s0)
@@ -340,6 +349,7 @@ subst_term sigma_term s = s :=
         (idSubst_term sigma_term Eq_term s1)
         (idSubst_term sigma_term Eq_term s2)
         (idSubst_term sigma_term Eq_term s3)
+  | tAlpha s0 => congr_tAlpha (idSubst_term sigma_term Eq_term s0)
   | tEmpty => congr_tEmpty
   | tEmptyElim s0 s1 =>
       congr_tEmptyElim
@@ -419,6 +429,7 @@ ren_term xi_term s = ren_term zeta_term s :=
         (extRen_term xi_term zeta_term Eq_term s1)
         (extRen_term xi_term zeta_term Eq_term s2)
         (extRen_term xi_term zeta_term Eq_term s3)
+  | tAlpha s0 => congr_tAlpha (extRen_term xi_term zeta_term Eq_term s0)
   | tEmpty => congr_tEmpty
   | tEmptyElim s0 s1 =>
       congr_tEmptyElim
@@ -503,6 +514,7 @@ subst_term sigma_term s = subst_term tau_term s :=
         (ext_term sigma_term tau_term Eq_term s1)
         (ext_term sigma_term tau_term Eq_term s2)
         (ext_term sigma_term tau_term Eq_term s3)
+  | tAlpha s0 => congr_tAlpha (ext_term sigma_term tau_term Eq_term s0)
   | tEmpty => congr_tEmpty
   | tEmptyElim s0 s1 =>
       congr_tEmptyElim
@@ -591,6 +603,8 @@ Fixpoint compRenRen_term (xi_term : nat -> nat) (zeta_term : nat -> nat)
         (compRenRen_term xi_term zeta_term rho_term Eq_term s1)
         (compRenRen_term xi_term zeta_term rho_term Eq_term s2)
         (compRenRen_term xi_term zeta_term rho_term Eq_term s3)
+  | tAlpha s0 =>
+      congr_tAlpha (compRenRen_term xi_term zeta_term rho_term Eq_term s0)
   | tEmpty => congr_tEmpty
   | tEmptyElim s0 s1 =>
       congr_tEmptyElim
@@ -690,6 +704,8 @@ subst_term tau_term (ren_term xi_term s) = subst_term theta_term s :=
         (compRenSubst_term xi_term tau_term theta_term Eq_term s1)
         (compRenSubst_term xi_term tau_term theta_term Eq_term s2)
         (compRenSubst_term xi_term tau_term theta_term Eq_term s3)
+  | tAlpha s0 =>
+      congr_tAlpha (compRenSubst_term xi_term tau_term theta_term Eq_term s0)
   | tEmpty => congr_tEmpty
   | tEmptyElim s0 s1 =>
       congr_tEmptyElim
@@ -805,6 +821,9 @@ ren_term zeta_term (subst_term sigma_term s) = subst_term theta_term s :=
         (compSubstRen_term sigma_term zeta_term theta_term Eq_term s1)
         (compSubstRen_term sigma_term zeta_term theta_term Eq_term s2)
         (compSubstRen_term sigma_term zeta_term theta_term Eq_term s3)
+  | tAlpha s0 =>
+      congr_tAlpha
+        (compSubstRen_term sigma_term zeta_term theta_term Eq_term s0)
   | tEmpty => congr_tEmpty
   | tEmptyElim s0 s1 =>
       congr_tEmptyElim
@@ -929,6 +948,9 @@ subst_term tau_term (subst_term sigma_term s) = subst_term theta_term s :=
         (compSubstSubst_term sigma_term tau_term theta_term Eq_term s1)
         (compSubstSubst_term sigma_term tau_term theta_term Eq_term s2)
         (compSubstSubst_term sigma_term tau_term theta_term Eq_term s3)
+  | tAlpha s0 =>
+      congr_tAlpha
+        (compSubstSubst_term sigma_term tau_term theta_term Eq_term s0)
   | tEmpty => congr_tEmpty
   | tEmptyElim s0 s1 =>
       congr_tEmptyElim
@@ -1095,6 +1117,7 @@ Fixpoint rinst_inst_term (xi_term : nat -> nat) (sigma_term : nat -> term)
         (rinst_inst_term xi_term sigma_term Eq_term s1)
         (rinst_inst_term xi_term sigma_term Eq_term s2)
         (rinst_inst_term xi_term sigma_term Eq_term s3)
+  | tAlpha s0 => congr_tAlpha (rinst_inst_term xi_term sigma_term Eq_term s0)
   | tEmpty => congr_tEmpty
   | tEmptyElim s0 s1 =>
       congr_tEmptyElim
